

\magnification=1800
\overfullrule=0pt
\parindent=0pt

\vsize=10 true in
\voffset=-.3 true in
\hsize=6.5 true in

\nopagenumbers

\input amstex

\def\ai{a^{-1}}
\def\bi{b^{-1}}
\def\ci{c^{-1}}

\input colordvi

\def\cltr{\Red}		  % Red  VERY-Approx PANTONE RED

\loadmsbm

\input epsf

\def\ctln{\centerline}
\def\u{\underbar}
\def\ssk{\smallskip}
\def\msk{\medskip}
\def\bsk{\bigskip}
\def\hsk{\hskip.1in}
\def\hhsk{\hskip.2in}
\def\dsl{\displaystyle}
\def\hskp{\hskip1.5in}

\def\lra{$\Leftrightarrow$ }
\def\ra{\rightarrow}
\def\mpto{\logmapsto}
\def\pu{\pi_1}
\def\mpu{$\pi_1$}
\def\sig{\Sigma}
\def\msig{$\Sigma$}
\def\ep{\epsilon}
\def\sset{\subseteq}
\def\del{\partial}
\def\inv{^{-1}}
\def\wtl{\widetilde}
%\def\lra{\Leftrightarrow}
\def\del{\partial}
\def\delp{\partial^\prime}
\def\delpp{\partial^{\prime\prime}}
\def\sgn{{\roman{sgn}}}
\def\wtih{\widetilde{H}}
\def\bbz{{\Bbb Z}}
\def\bbr{{\Bbb R}}
\def\rtar{$\Rightarrow$}

\def\cltr{\Red}		  % Red  VERY-Approx PANTONE RED
\def\cltb{\Blue}		  % Blue  Approximate PANTONE BLUE-072
\def\cltg{\PineGreen}	  % ForestGreen  Approximate PANTONE 349

\hskip-.2in {\bf Another non-trivial presentation of the trivial group}

\bsk

$G=\langle a,b,c\ |\ bba\bi\ai,ccb\ci\bi,aac\ai\ci\rangle $

$= \langle a,b,c\ |\ ab\ai=b^2,bc\bi=c^2,ca\ci=a^2\rangle$


\msk

Then:
\hsk
$ab\ai=b^2$, so $(ab\ai)^{-1} =a\bi\ai =b^{-2}$, 

so $a\bi=b^{-2}a$.
\hsk
Also, 

$b^2a=ab$, so $ba\bi=\bi(b^2a)b=\bi(ab)\bi = \bi a$.

\underbar{Also}, 

$b^2ab^{-2}=b(ba\bi)\bi =b\bi a\bi=a\bi =b^{-2}a$.

\ssk

Similarly, $c^2b=bc$, so $cb=\ci bc$, and $c^2bc^{-2}=c^{-2}b$.

\msk

\underbar{Then}: $ca\ci=a^2$, so $b(ca\ci)\bi=b(a^2)\bi$. But

\ssk

$b(ca\ci)\bi=(bc)a(bc)^{-1}=(c^2b)a(c^2b)^{-1}
=c^2(ba\bi)c^{-2}$

$=c^2(\bi a)c^{-2}=(c^2\bi c^{-2})(c^2ac^{-2})$

$=(c^2bc^{-2})^{-1}c(ca\ci)\ci=(c^{-2}b)^{-1}c(a^2)\ci$

$=\bi c^2(ca\ci)^2=\bi c^2(a^2)^2=\bi c^2a^4$

and

$b(a^2)\bi=(ba\bi)^2=(\bi a)^2=\bi a\bi a
=\bi(a\bi)a$

$=\bi(b^{-2}a)a=b^{-3}a^2$,

so $\bi c^2a^4=b^{-3}a^2$, 

so $c^2=b(\bi c^2a^4)a^{-4}=b(b^{-3}a^2)a^{-4}=b^{-2}a^{-2}$.

So $c^{-2}=(c^2)^{-1}=(b^{-2}a^{-2})^{-1}=a^2b^2$.

\msk

\underbar{Then} $bc=\ci(cb)c=\ci(\ci bc)c=c^{-2}bc^2$

$=(a^2b^2)b(b^{-2}a^{-2})=a^2ba^{-2}=a(ab\ai)\ai$

$=ab^2\ai=(ab\ai)^2=(b^2)^2=b^4$, 

so $c=\bi(bc)=\bi(b^4)=b^3$.

\msk

So $b^6=c^2=bc\bi=bb^3\bi=b^3$. So $b^3=1$, so $c=1$.

\ssk

Then $a^2=ca\ci=a$, so $a=1$; 

and then $b^2=ab\ai=b$, so $b=1$.

\msk

Consequently, $a=b=c=1$, so $G=\{1\}$.

\vfill
\end





$aaab\ai\bi\ai=$
\hhsk
